reduced complexity

theories/CADP.v
@@ -18,14 +18,14 @@ end.
 (**** Basic defs *********************************************************)
 (*************************************************************************)
 
-Definition index : Type := option nat.
-Definition pid   : Type := nat.
 
-Definition ibool : Type := nat.
-Definition iloop : Type := nat.
-
+(* pid is a non-nil index *)
+Definition pid   : Type  := nat.
+Definition index : Type  := option pid.
 Definition Nil   : index := None.
 
+(* loop identifier *)
+Definition iloop : Type := nat.
 
 (* we dont need new_i, only i and j *)
 Definition lock : Type := index * index.
@@ -41,16 +41,10 @@ Module Index.
 
   Definition of_pid (i : pid) : index := Some i.
 
-  Definition to_nat (i : index) : nat :=
-    match i with
-    | None => 0
-    | Some n => n
-    end.
-
   Definition is_nil (i : index) : bool :=
     match i with
-    | None => false
-    | _ => true
+    | None => true
+    | _ => false
     end.
 
   Definition eqb (i:index) (j:index) : bool :=
@@ -60,41 +54,7 @@ Module Index.
     | _, _ => false
     end.
 
-  Definition is_index (n:option nat) : bool := true.
-
 End Index.
-
-
-Module PID.
-
-  Definition is_pid (n : nat) : bool := if Nat.eqb n 0 then false else true.
-
-  Definition to_nat (p:pid) : nat := p.
-
-End PID.
-
-
-
-Module IBool.
-
-  Definition of_bool (b:bool) : ibool := if b then 1 else 0.
-
-  Definition to_nat (b:ibool) : nat := b.
-
-  Definition is_ibool (n:nat) : bool :=
-    match n with
-    | 0 => true
-    | 1 => true
-    | _ => false
-    end.
-
-  Definition is_some (b:option ibool) : bool :=
-    match b with
-    | None => false
-    | _    => true
-    end.
-
-End IBool.
 
 
 
@@ -102,926 +62,605 @@ End IBool.
 (*************************************************************************)
 (**** Memory *************************************************************)
 (*************************************************************************)
+
+
+(**********************************)
+(**** Qnode ***********************)
+(**********************************)
+
+Record qnode :=
+  { next   : index
+  ; locked : bool }.
+
+Module Qnode.
+  Definition initial : qnode := Build_qnode Nil false.
+
+  Definition get_next   (q:qnode) : index := next q.
+  Definition get_locked (q:qnode) : bool  := locked q.
+
+  Definition set_next   (i:index) (q:qnode) : qnode := Build_qnode
+                                                        i (Qnode.get_locked q).
+  Definition set_locked (b:bool)  (q:qnode) : qnode := Build_qnode
+                                                        (Qnode.get_next q) b.
+End Qnode.
+
+
+(**********************************)
+(**** mem (Memory) Type ***********)
+(**********************************)
+
+Definition mem : Type := list qnode.
+
+Fixpoint mem_create (n:nat) : mem :=
+  match n with
+  | 0    => []
+  | S n' => app (mem_create n') [Qnode.initial]
+  end.
+
 Module Memory.
+  Definition initial  (n:nat) : mem := mem_create n.
 
-  (**********************************)
-  (**** Qnode ***********************)
-  (**********************************)
+  Definition nth_error (i:nat) (m:mem) : option qnode := nth_error m i.
 
-  Record qnode :=
-    { next   : index
-    ; locked : ibool }.
+  Definition nth_default (d:qnode) (i:nat) (m:mem) : qnode := nth_default d m i.
 
-  Module Qnode.
-    Definition initial : qnode := Build_qnode Nil 0.
-
-    Module _Get.
-      Definition next   (q:qnode) : index := (next q).
-      Definition locked (q:qnode) : ibool := (locked q).
-    End _Get.
-
-
-    Module _Set.
-      Definition next   (i:index) (q:qnode) : qnode :=
-        Build_qnode i (Qnode._Get.locked q).
-      Definition locked (b:ibool) (q:qnode) : qnode :=
-        Build_qnode (Qnode._Get.next q) b.
-    End _Set.
-
-  End Qnode.
-
-
-  (**********************************)
-  (**** mem Type & app **************)
-  (**********************************)
-
-  Definition mem : Type := list qnode.
-
-  (**********************************)
-  (**** Creating & Initializing *****)
-  (**********************************)
-
-  Fixpoint create (n:nat) : mem :=
-    match n with
-    | 0    => []
-    | S n' => app (create n') [Qnode.initial]
-    end.
-
-  Definition initial (n:nat) : mem := create n.
-
-  (**********************************)
-  (**** helpful funs/definitions ****)
-  (**********************************)
-
-  Fixpoint length_of (m:mem) : nat :=
-    match m with
-    | [] => 0
-    | h :: t => S (length_of t)
-    end.
-
-  Fixpoint add_n_qnodes (n:nat) (m:mem) :=
-    match n with
-      | O  => m
-      | S n' => Qnode.initial::(add_n_qnodes n' m)
-    end.
-
-  (* pads mem so that index i exists *)
-  Definition pad (i:nat) (m:mem) : mem :=
-    let length_of_m:nat := length_of m in
-    if (Nat.ltb length_of_m i)
-    then (add_n_qnodes (i - length_of_m) m)
-    else m.
-
-
-  Module _Get.
-
-
-    Definition index_of (i:nat) (m:mem) := nth_error m i.
-
-    Definition locked_of (i:index) (m:mem) : option ibool :=
-      match i with
+  Fixpoint nth_replace (r:qnode) (i:nat) (m:mem) : option mem :=
+    match i, m with
+    | 0, [] => None
+    | 0, h :: t => Some (r :: t)
+    | S n, [] => None
+    | S n, h :: t =>
+      match nth_replace r n m with
       | None => None
-      | Some n =>
-        match (index_of n m) with
-        | None => None
-        | Some b => Some (locked b)
-        end
-      end.
+      | Some t' => Some (h :: t')
+      end
+    end.
 
-    Definition next_of (i:index) (m:mem) : index :=
-      match i with
-        | None => None
-        | Some n =>
-        match (index_of n m) with
-        | None => None
-        | Some b => next b
-        end
-      end.
-
-  End _Get.
-
-
-  Module _Set.
-
-    Fixpoint index_of (i:nat) (q:qnode) (m:mem) : option mem :=
-      match m with
-      | []     => None
-      | h :: t =>
-        let length_of_m:nat := length_of m in
-        match i, length_of_m with
-        | _, 0 => None
-        | _, _ =>
-          if (Nat.eqb i length_of_m) then Some (q :: t)
-          else match (index_of i q t) with
-               | None   => None
-               | Some l => Some (h :: l)
-               end
-        end
-      end.
-
-    Definition locked_of (i:index) (l:ibool) (m:mem) : option mem :=
-      match i with
-        | None => None
-        | Some n =>
-        match _Get.index_of n m with
-        | None       => None
-        | Some qnode => index_of n (Qnode._Set.locked l qnode) m
-        end
-      end.
-
-    Definition next_of (i:index) (n:index) (m:mem) : option mem :=
-      match i with
-      | None => None
-      | Some j =>
-        match _Get.index_of j m with
-        | None       => None
-        | Some qnode => index_of j (Qnode._Set.next n qnode) m
-        end
-      end.
-
-  End _Set.
 End Memory.
 
 
+
 (*************************************************************************)
-(**** Vars ***************************************************************)
+(**** Vars (Local to process ) *******************************************)
 (*************************************************************************)
+
+Record local_vars :=
+  { var_predecessor : index (* acquire *)
+  ; var_locked      : bool  (* acquire *)
+  ; var_next        : index (* release *)
+  ; var_swap        : bool  (* release *) }.
+
 Module Vars.
-
-  Record vars :=
-  { var_predecessor : index        (* acquire *)
-  ; var_locked      : option ibool (* acquire *)
-  ; var_next        : index        (* release *)
-  ; var_swap        : option ibool (* release *) }.
-
-  Definition initial : vars := Build_vars None None None None.
-
-  Inductive var : Type :=
-    | PREDECESSOR
-    | LOCKED
-    | NEXT
-    | SWAP
-    | PID
-    (* | NIL *)
-    .
-
-
-  Module Kind.
-    Inductive kind : Type := | INDEX | IBOOL | PID.
-  End Kind.
-
-
-  Module _Get.
-
-    Definition predecessor (v:vars) : index := var_predecessor v.
-
-    Definition locked (v:vars) : option ibool := var_locked v.
-
-    Definition next (v:vars) : index := var_next v.
-
-    Definition swap (v:vars) : option ibool := var_swap v.
-
-  End _Get.
-
-
-  Module _Set.
-
-    Definition predecessor (i:index) (v:vars) : vars :=
-      Build_vars i (_Get.locked v) (_Get.next v) (_Get.swap v).
-
-    Definition locked (b:ibool) (v:vars) : vars :=
-      Build_vars (_Get.predecessor v) (Some b) (_Get.next v) (_Get.swap v).
-
-    Definition next (i:index) (v:vars) : vars :=
-      Build_vars (_Get.predecessor v) (_Get.locked v) i (_Get.swap v).
-
-    Definition swap (b:ibool) (v:vars) : vars :=
-      Build_vars (_Get.predecessor v) (_Get.locked v) (_Get.next v) (Some b).
-
-  End _Set.
-
+  Definition initial : local_vars := Build_local_vars None false None false.
 End Vars.
+
+Inductive local_var : Type :=
+  | VAR_PREDECESSOR
+  | VAR_LOCKED
+  | VAR_NEXT
+  | VAR_SWAP
+  | VAR_PID
+  .
+
+Definition set_predecessor (i:index) (v:local_vars) : local_vars :=
+  Build_local_vars i (var_locked v) (var_next v) (var_swap v).
+
+Definition set_locked (b:bool) (v:local_vars) : local_vars :=
+  Build_local_vars (var_predecessor v) b (var_next v) (var_swap v).
+
+Definition set_next (i:index) (v:local_vars) : local_vars :=
+  Build_local_vars (var_predecessor v) (var_locked v) i (var_swap v).
+
+Definition set_swap (b:bool) (v:local_vars) : local_vars :=
+  Build_local_vars (var_predecessor v) (var_locked v) (var_next v) b.
+
+
 
 
 (*************************************************************************)
 (**** Value **************************************************************)
 (*************************************************************************)
-Module Val.
-  Inductive val : Type :=
-  | INDEX : index        -> val
-  | IBOOL : option ibool -> val
-  | PID : val
-  | VAR : Vars.var -> val
-  | TRU : val
-  | FLS : val
-  | NIL : val
-  .
-End Val.
 
+(* FIXME: David mentioned to use [Set] instead of [Type] here,
+but it returned [Universal inconsistency, cannot enforce pid.u0<=Set] *)
+Inductive value : Type (*Set*) :=
+  | NAT : nat -> value
+  | PID : pid -> value
+  | INDEX : index -> value
+  | BOOL : bool -> value
+  | NIL : value
+  .
+
+
+Definition valid_cast_to_nat (v:value) : bool * option nat :=
+  match v with
+  | NAT n => (true, Some n)
+  | PID p => (true, Some p)
+  | INDEX i => (true, i)
+  | _ => (false, None) (* i.e., BOOL, NIL *)
+  end.
 
 (*************************************************************************)
 (**** (Global) Resource **************************************************)
 (*************************************************************************)
+Definition resource : Type := mem * lock.
+
 Module Resource.
-  Definition resource : Type := Memory.mem * lock.
   Definition initial (n:nat) : resource := (Memory.initial n, Lock.initial).
 
-  Module _Get.
-    Definition mem (s:resource) : Memory.mem :=
-      match s with
-      | (mem, lock) => mem
-      end.
+  Definition get_mem (r:resource) : mem :=
+    match r with | (m, _) => m end.
 
-    Definition lock (s:resource) : lock :=
-      match s with
-      | (mem, lock) => lock
-      end.
+  Definition get_lock_i (r:resource) : index :=
+    match r with | (_, (i, _)) => i end.
 
-    Module Lock.
-      Definition i (s:resource) : index :=
-        match (lock s) with
-        | (i, j) => i
-        end.
+  Definition get_lock_j (r:resource) : index :=
+    match r with | (_, (_, j)) => j end.
 
-      Definition j (s:resource) : index :=
-        match (lock s) with
-        | (i, j) => j
-        end.
+  Definition set_mem (new_m:mem) (r:resource) : resource :=
+    match r with | (_, l) => (new_m, l) end.
 
-    End Lock.
-  End _Get.
+  Definition set_lock_i (new_i:index) (r:resource) : resource :=
+    match r with | (m, (_, j)) => (m, (new_i, j)) end.
 
-
-  Module _Set.
-    Module Lock.
-      Definition i (new_i:index) (s:resource) : resource :=
-        match (_Get.lock s) with
-        | (i, j) => (_Get.mem s, (new_i, j))
-        end.
-
-      Definition j (new_j:index) (s:resource) : resource :=
-        match (_Get.lock s) with
-        | (i, j) => (_Get.mem s, (i, new_j))
-        end.
-
-    End Lock.
-  End _Set.
+  Definition set_lock_j (new_j:index) (r:resource) : resource :=
+    match r with | (m, (i, _)) => (m, (i, new_j)) end.
 End Resource.
 
 
 (*************************************************************************)
 (**** (Local) State ******************************************************)
 (*************************************************************************)
+Definition state : Type := pid * local_vars.
+
 Module State.
+  Definition create (p:pid) : state := (p, Vars.initial).
+  Definition initial : state := State.create 0.
 
-  Definition local : Type := pid * Vars.vars.
+  Definition get_pid (s:state) : pid :=
+    match s with | (p, _) => p end.
 
-  Definition create (p:pid) : local := (p, Vars.initial).
+  Definition get_vars (s:state) : local_vars :=
+    match s with | (_, v) => v end.
 
-  Module _Get.
-    Definition pid (s:local) : pid :=
-      match s with
-      | (pid, vars) => pid
-      end.
+  Definition get_predecessor (s:state) : index := var_predecessor (get_vars s).
+  Definition get_locked      (s:state) : bool  := var_locked (get_vars s).
+  Definition get_next        (s:state) : index := var_next (get_vars s).
+  Definition get_swap        (s:state) : bool  := var_swap (get_vars s).
 
-    Definition vars (s:local) : Vars.vars :=
-      match s with
-      | (pid, vars) => vars
-      end.
+  Definition get_local_var_value (v:local_var) (s:state) : value :=
+    match v with
+    | VAR_PREDECESSOR => INDEX (get_predecessor s)
+    | VAR_LOCKED      => BOOL  (get_locked s)
+    | VAR_NEXT        => INDEX (get_next s)
+    | VAR_SWAP        => BOOL  (get_swap s)
+    | VAR_PID         => PID   (get_pid s)
+    end.
 
+  Definition set_vars (v:local_vars) (s:state) : state :=
+    match s with | (p, _) => (p, v) end.
 
-    Module Var.
-      Definition predecessor (s:local) : index :=
-        Vars._Get.predecessor (vars s).
-      Definition locked (s:local) : option ibool := Vars._Get.locked (vars s).
-      Definition next (s:local) : index := Vars._Get.next (vars s).
-      Definition swap (s:local) : option ibool := Vars._Get.swap (vars s).
-
-    End Var.
-
-    Definition var (v:Vars.var) (s:local) : option nat :=
-      match v with
-      | Vars.PREDECESSOR => Var.predecessor s
-      | Vars.LOCKED      => Var.locked s
-      | Vars.NEXT        => Var.next s
-      | Vars.SWAP        => Var.swap s
-      | Vars.PID         => Some (pid s)
-      end.
-
-    Definition val (v:Val.val) (s:local) : option nat :=
-      match v with
-      | Val.INDEX i => i
-      | Val.IBOOL b => b
-      | Val.PID     => Some (pid s)
-      | Val.VAR v   => var v s
-      | Val.TRU     => Some 1
-      | Val.FLS     => Some 0
-      | Val.NIL     => Nil
-      end.
-
-  End _Get.
-
-
-  Module _Set.
-    Module Var.
-
-      Definition predecessor (i:index) (s:local) : local :=
-        match s with
-        | (pid, vars) => (pid, Vars._Set.predecessor i vars)
-        end.
-
-      Definition locked (b:ibool) (s:local) : local :=
-        match s with
-        | (pid, vars) => (pid, Vars._Set.locked b vars)
-        end.
-
-      Definition next (i:index) (s:local) : local :=
-        match s with
-        | (pid, vars) => (pid, Vars._Set.next i vars)
-        end.
-
-      Definition swap (b:ibool) (s:local) : local :=
-        match s with
-        | (pid, vars) => (pid, Vars._Set.swap b vars)
-        end.
-
-    End Var.
-  End _Set.
 End State.
 
 
 (*************************************************************************)
 (**** Environment (local) ************************************************)
 (*************************************************************************)
-Definition env : Type := State.local * Resource.resource.
+Definition env : Type := state * resource.
 
 Module Env.
-  Module _Get.
 
-    Definition local (e:env) : State.local :=
-      match e with | (l, r) => l end.
+  Definition get_state (e:env) : state := match e with | (s, _) => s end.
 
-    Definition pid (e:env) : pid := State._Get.pid (local e).
-    Definition vars (e:env) : Vars.vars := State._Get.vars (local e).
+  Definition get_resource (e:env) : resource := match e with | (_, r) => r end.
 
-    Module Var.
-      Definition predecessor (e:env) : index :=
-        Vars._Get.predecessor (vars e).
-      Definition locked (e:env) : option ibool :=
-        Vars._Get.locked (vars e).
-      Definition next (e:env) : index :=
-        Vars._Get.next (vars e).
-      Definition swap (e:env) : option ibool :=
-        Vars._Get.swap (vars e).
+  Definition set_state (s:state) (e:env) : env :=
+    match e with | (_, r) => (s, r) end.
 
-    End Var.
-
-    Definition var (v:Vars.var) (e:env) : option nat :=
-      State._Get.var v (local e).
-
-    Definition val (v:Val.val) (e:env) : option nat :=
-      State._Get.val v (local e).
-
-    Definition resource (e:env) : Resource.resource :=
-      match e with | (l, r) => r end.
-
-    Definition mem (e:env) : Memory.mem :=
-      Resource._Get.mem (resource e).
-
-    Module Mem.
-      Definition locked_of (i:index) (e:env) : option ibool :=
-        Memory._Get.locked_of i (Env._Get.mem e).
-
-      Definition next_of (i:index) (e:env) : index :=
-        Memory._Get.next_of i (Env._Get.mem e).
-
-    End Mem.
-
-
-    Definition lock (e:env) : lock :=
-      Resource._Get.lock (resource e).
-
-    Module Lock.
-      Definition i (e:env) : index :=
-        Resource._Get.Lock.i (Env._Get.resource e).
-      Definition j (e:env) : index :=
-        Resource._Get.Lock.j (Env._Get.resource e).
-
-    End Lock.
-  End _Get.
-
-
-  Module _Set.
-    Module Var.
-
-      Definition predecessor (i:index) (e:env) : env :=
-        match e with
-        | (l, r) => ((State._Set.Var.predecessor i l), r)
-        end.
-
-      Definition locked (b:ibool) (e:env) : env :=
-        match e with
-        | (l, r) => ((State._Set.Var.locked b l), r)
-        end.
-
-      Definition next (i:index) (e:env) : env :=
-        match e with
-        | (l, r) => ((State._Set.Var.next i l), r)
-        end.
-
-      Definition swap (b:ibool) (e:env) : env :=
-        match e with
-        | (l, r) => ((State._Set.Var.swap b l), r)
-        end.
-
-    End Var.
-
-    Definition resource (r:Resource.resource) (e:env) : env :=
-      (Env._Get.local e, r).
-
-    Definition mem (m:Memory.mem) (e:env) : env :=
-      (Env._Get.local e, (m, Env._Get.lock e)).
-
-    Module Mem.
-      Definition locked_of (i:index) (b:ibool) (e:env) : option env :=
-        match (Memory._Set.locked_of i b (Env._Get.mem e)) with
-        | None => None
-        | Some m => Some (mem m e)
-        end.
-
-      Definition next_of (i:index) (n:index) (e:env) : option env :=
-        match (Memory._Set.next_of i n (Env._Get.mem e)) with
-        | None => None
-        | Some m => Some (mem m e)
-        end.
-
-    End Mem.
-
-    Definition lock (l:lock) (e:env) : env :=
-      (Env._Get.local e, (Env._Get.mem e, l)).
-
-    Module Lock.
-      Definition i (new_i:index) (e:env) : env :=
-        resource (Resource._Set.Lock.i new_i (Env._Get.resource e)) e.
-
-      Definition j (new_j:index) (e:env) : env :=
-        resource (Resource._Set.Lock.j new_j (Env._Get.resource e)) e.
-
-    End Lock.
-
-  End _Set.
-
-
-  Module Handle.
-
-    (** [read_next e] will set var [next] to be the value
-        currently of the [qnode.next] corresponding to the
-        [pid] of the process in the state. *)
-    Definition read_next (e:env) : env :=
-      let p : pid        := Env._Get.pid e in
-      let new_next:index := Env._Get.Mem.next_of (Index.of_pid p) e in
-      Env._Set.Var.next new_next e.
-
-    (** [read_locked e] will set var [locked] to be
-        the value of the [qnode.locked] corresponding
-        to the [pid] of the process in the state.
-        ! ! ! it requires that [qnode.locked] is not None. *)
-    Definition read_locked (e:env) : env :=
-    let p : pid        := Env._Get.pid e in
-    match (Env._Get.Mem.locked_of (Index.of_pid p) e) with
-    | None => e (* shouldn't happen, semantics guard from this. *)
-    | Some new_locked => Env._Set.Var.locked new_locked e
-    end.
-
-    (*  *)
-    Definition write_next (to_write:Vars.var) (next:Val.val) (e:env) : env :=
-      match (Env._Get.val next e) with
-      | None => e (* shouldn't happen, semantics guard from this. *)
-      | Some next' =>
-        let next' : index := Index.of_pid next' in
-        match (Env._Get.var to_write e) with
-        | None => e (* shouldn't happen, semantics guard from this. *)
-        | Some to_write' =>
-          match (Env._Set.Mem.next_of (Index.of_pid to_write') next' e) with
-          | None => e (* shouldn't happen, semantics guard from this. *)
-          | Some e' => e'
-          end
-        end
-      end.
-
-    (*  *)
-    Definition write_locked (to_write:Vars.var) (locked:Val.val) (e:env) : env :=
-      match (Env._Get.val locked e) with
-        | None => e (* shouldn't happen, semantics guard from this. *)
-        | Some locked' =>
-        match (IBool.is_ibool locked') with
-        | false => e (* shouldn't happen, semantics guard from this. *)
-        | true =>
-          match (Env._Get.var to_write e) with
-          | None => e (* shouldn't happen, semantics guard from this. *)
-          | Some to_write' =>
-            let to_write' : index := Index.of_pid to_write' in
-            match (Env._Set.Mem.locked_of to_write' locked' e) with
-            | None => e (* shouldn't happen, semantics guard from this. *)
-            | Some e' => e'
-            end
-          end
-        end
-      end.
-
-    (*  *)
-    Definition fetch_and_store (e:env) : env :=
-      (* store [Lock.i] in [Vars.predecessor]. *)
-      let i : index := Env._Get.Lock.i e in
-      let e' : env := Env._Set.Var.predecessor i e in
-      (* set [Lock.i] to [pid]. *)
-      let p : pid := Env._Get.pid e' in
-      Env._Set.Lock.i (Index.of_pid p) e'.
-
-    (*  *)
-    Definition compare_and_swap (e:env) : env :=
-      let i : index := Env._Get.Lock.i e in
-      let j : index := Env._Get.Lock.j e in
-      (* set [Lock.j] to [pid]. *)
-      let p : pid := Env._Get.pid e in
-      let e' : env := Env._Set.Lock.j (Index.of_pid p) e in
-      let are_eq : bool := Index.eqb i j in
-      Env._Set.Var.swap
-        (IBool.of_bool are_eq)
-        (* also, if eq then reset [i] to Nil. *)
-        (if are_eq then Env._Set.Lock.i Nil e' else e').
-
-    End Handle.
+  Definition set_resource (r:resource) (e:env) : env :=
+    match e with | (s, _) => (s, r) end.
 
 End Env.
 
 
 
 (*************************************************************************)
+(**** (Conditional) Expressions ******************************************)
+(*************************************************************************)
+
+Inductive expr : Type :=
+  | NOT : expr -> expr
+  | EQ : expr -> expr -> expr
+  | VAR : local_var -> expr
+  | VAL : value -> expr
+  | TRU : expr
+  | FLS : expr
+  .
+
+Module Expr.
+  Definition of_bool (b:bool) : expr := if b then TRU else FLS.
+End Expr.
+
+Fixpoint eval (e:expr) (s:state) : option expr :=
+  match e with
+
+  | NOT b =>
+    match eval b s with
+    | Some TRU => Some FLS
+    | Some FLS => Some TRU
+    | _ => None
+    end
+
+  | EQ a b =>
+    match eval a s, eval b s with
+    | Some (VAL (NAT a)),
+      Some (VAL (NAT b))   => Some (Expr.of_bool (Nat.eqb a b))
+
+    | Some (VAL (INDEX a)),
+      Some (VAL (INDEX b)) => Some (Expr.of_bool (Index.eqb a b))
+
+    | Some (VAL (PID a)),
+      Some (VAL (PID b))   => Some (Expr.of_bool (Nat.eqb a b))
+
+    | Some (VAL (BOOL a)),
+      Some (VAL (BOOL b))  => Some (Expr.of_bool (eqb a b))
+
+    | _, _ => None
+    end
+
+  | VAR v => Some (VAL (State.get_local_var_value v s))
+
+  | VAL v => Some (VAL v)
+
+  | TRU => Some TRU
+  | FLS => Some FLS
+  end.
+
+
+(*************************************************************************)
+(**** Actions ************************************************************)
+(*************************************************************************)
+
+Inductive act : Type :=
+  | NCS   : act
+  | ENTER : act
+  | LEAVE : act
+
+  | READ_NEXT   : act
+  | READ_LOCKED : act
+
+  (* below: [expr] as may be value or var *)
+  | WRITE_NEXT   : local_var -> expr -> act
+  | WRITE_LOCKED : local_var -> expr -> act
+
+  | FETCH_AND_STORE  : act
+  | COMPARE_AND_SWAP : act
+  .
+
+
+(*************************************************************************)
 (**** Process ************************************************************)
 (*************************************************************************)
-Module Process.
 
-  Module Expr.
+Inductive tm : Type :=
+  | ERR : tm (* error *)
+  | OK  : tm (* no-op *)
+  | END : tm (* termination *)
 
-    Inductive value : Set :=. (*TODO Move values from [expr] to [value]*)
+  | IF  : expr -> tm -> tm -> tm
 
-    Inductive expr : Type :=
-      | NOT : expr -> expr
-      | VAR : Vars.var -> expr
-      | NAT : nat -> expr
-      | IBOOL : ibool -> expr
-      | INDEX : index -> expr
-      | CAST : expr -> Vars.Kind.kind -> expr
-      | PID : pid -> expr
-      | EQ  : expr -> expr -> expr
-      | TT  : expr
-      | FF  : expr
-      | NIL : expr
-      .
+  | ACT : act -> tm
 
-    Inductive eval : (expr * env) -> (expr * env) -> Prop :=
+  | SEQ : tm -> tm -> tm
 
-      | IBOOL_TT : forall e, eval (IBOOL 1, e) (TT, e)
-      | IBOOL_FF : forall e, eval (IBOOL 0, e) (FF, e)
+  | LOOP      : tm -> tm (* inner loop body -> *)
+  | LOOP_END  : tm
 
-      | NOT_TT : forall e, eval (NOT TT, e) (FF, e)
-      | NOT_FF : forall e, eval (NOT FF, e) (TT, e)
+  (* loop id -> body -> outer continuation -> ... *)
+  | LOOP_OVER : iloop -> tm -> tm -> tm
+  | BREAK     : iloop -> tm
+  .
 
-      | VAR_PREDECESSOR : forall e,
-        eval
-          (VAR Vars.PREDECESSOR, e)
-          (INDEX (Env._Get.Var.predecessor e), e)
+Declare Custom Entry tm.
+Declare Scope tm_scope.
+Notation "<{ e }>" := e (e custom tm at level 99): tm_scope.
+Notation "( x )" := x (in custom tm, x at level 99): tm_scope.
+Notation "x" := x (in custom tm at level 0, x constr at level 0): tm_scope.
+Notation "'if' c 'then' t 'else' e" := (IF c t e)
+                (in custom tm at level 90, c custom tm at level 80,
+                  t custom tm at level 80, e custom tm at level 80): tm_scope.
+Local Open Scope tm_scope.
 
-      | VAR_LOCKED : forall v b e,
-        (Env._Get.Var.locked e)=v /\ v=(Some b) ->
-        eval (VAR Vars.LOCKED, e) (IBOOL b, e)
+Fixpoint subst (new old:tm) (loops:bool) : tm :=
+  match old with
+  | ERR => ERR
+  | OK   => OK
+  | END   => END
 
-      | VAR_NEXT : forall v e,
-        (Env._Get.Var.next e)=v ->
-        eval (VAR Vars.NEXT, e) (INDEX v, e)
+  | IF c t e => IF c (subst new t loops) (subst new e loops)
 
-      | VAR_SWAP : forall v b e,
-        (Env._Get.Var.swap e)=v /\ v=(Some b) ->
-        eval (VAR Vars.SWAP, e) (IBOOL b, e)
+  | ACT a => ACT a
 
-      | CAST_PID_TO_INDEX : forall p e,
-        eval (CAST (PID p) Vars.Kind.INDEX, e) (INDEX (Index.of_pid p), e)
+  (* do not substitute in other body *)
+  | SEQ l r => SEQ l (subst new r loops)
 
-      | CAST_INDEX_TO_PID : forall i n e,
-        (i=Some(S n)) ->
-        eval (CAST (INDEX i) Vars.Kind.PID, e) (PID n, e)
+  | LOOP b   => if loops then LOOP (subst new b loops) else LOOP b
+  | LOOP_END => new
 
-      | EQ_TT_NAT : forall n m e,
-        (Nat.eqb n m)=true ->
-        eval (EQ (NAT n) (NAT m), e) (TT, e)
-
-      | EQ_FF_NAT : forall n m e,
-        (Nat.eqb n m)=false ->
-        eval (EQ (NAT n) (NAT m), e) (FF, e)
-
-      | EQ_TT_IBOOL : forall n m e,
-        ((IBool.is_ibool n)=true /\ (IBool.is_ibool m)=true)
-        /\ (Nat.eqb (IBool.to_nat n) (IBool.to_nat m))=true ->
-        eval (EQ (IBOOL n) (IBOOL m), e) (TT, e)
-
-      | EQ_FF_IBOOL : forall n m e,
-        ((IBool.is_ibool n)=false \/ (IBool.is_ibool m)=false)
-        \/ (Nat.eqb (IBool.to_nat n) (IBool.to_nat m))=false ->
-        eval (EQ (IBOOL n) (IBOOL m), e) (FF, e)
-
-      | EQ_TT_INDEX : forall n m e,
-        (Nat.eqb (Index.to_nat n) (Index.to_nat m))=true ->
-        eval (EQ (INDEX n) (INDEX m), e) (TT, e)
-
-      | EQ_FF_INDEX : forall n m e,
-        (Nat.eqb (Index.to_nat n) (Index.to_nat m))=false ->
-        eval (EQ (INDEX n) (INDEX m), e) (TT, e)
-
-      | EQ_TT_PID : forall n m e,
-        ((PID.is_pid n)=true /\ (PID.is_pid m)=true)
-        /\ (Nat.eqb (PID.to_nat n) (PID.to_nat m))=true ->
-        eval (EQ (PID n) (PID m), e) (TT, e)
-
-      | EQ_FF_PID : forall n m e,
-        ((PID.is_pid n)=false \/ (PID.is_pid m)=false)
-        \/ (Nat.eqb (PID.to_nat n) (PID.to_nat m))=false ->
-        eval (EQ (PID n) (PID m), e) (TT, e)
-
-      | EQ_TT_NIL_NIL : forall e,
-        eval (EQ NIL NIL, e) (TT, e)
-
-      | EQ_TT_NIL_INDEX_L : forall n e,
-        (Index.is_nil n)=true ->
-        eval (EQ (INDEX n) NIL, e) (TT, e)
-
-      | EQ_FF_NIL_INDEX_L : forall n e,
-        (Index.is_nil n)=false ->
-        eval (EQ (INDEX n) NIL, e) (FF, e)
-
-      | EQ_TT_NIL_INDEX_R : forall n e,
-        (Index.is_nil n)=true ->
-        eval (EQ NIL (INDEX n), e) (TT, e)
-
-      | EQ_FF_NIL_INDEX_R : forall n e,
-        (Index.is_nil n)=false ->
-        eval (EQ NIL (INDEX n), e) (FF, e)
-
-      | EQ_FF_NIL_PID_L : forall n e,
-        (PID.is_pid n)=true ->
-        eval (EQ (PID n) NIL, e) (FF, e)
-
-      | EQ_FF_NIL_PID_R : forall n e,
-        (PID.is_pid n)=true ->
-        eval (EQ NIL (PID n), e) (FF, e)
-      .
-
-    Print eval.
-
-  End Expr.
+  | LOOP_OVER l b c => LOOP_OVER l (subst new b loops) (subst new c loops)
+  | BREAK l         => BREAK l
+  end.
 
 
-  Module Operation.
+(*************************************************************************)
+(**** (Local) Semantics of Processes *************************************)
+(*************************************************************************)
 
-    (* used in steps, not syntax *)
-    Inductive act : Type :=
-      | NCS   : act
-      | ENTER : act
-      | LEAVE : act
+(** [read_next e] will set var [next] to be the value
+    currently of the [qnode.next] corresponding to the
+    [pid] of the process in the state. *)
+Definition read_next (e:env) : option env :=
+  (* get pid *)
+  let s:state := Env.get_state e in
+  let p:pid := State.get_pid s in
+  (* get qnode *)
+  let r:resource := Env.get_resource e in
+  let m:mem := Resource.get_mem r in
+  match Memory.nth_error p m with
+  | None => None (* tried to access out of bounds *)
+  | Some q => (* get next of qnode *)
+    let qnode_next:index := Qnode.get_next q in
+    (* get local vars *)
+    let v:local_vars := State.get_vars s in
+    (* update env *)
+    let e:env := Env.set_state (State.set_vars (set_next qnode_next v) s) e in
+    Some e
+  end.
 
-      | READ_NEXT   : act
-      | READ_LOCKED : act
+(** [read_locked e] will set var [locked] to be
+    the value of the [qnode.locked] corresponding
+    to the [pid] of the process in the state.
+    ! ! ! it requires that [qnode.locked] is not None. *)
+Definition read_locked (e:env) : option env :=
+  (* get pid *)
+  let s:state := Env.get_state e in
+  let p:pid := State.get_pid s in
+  (* get qnode *)
+  let r:resource := Env.get_resource e in
+  let m:mem := Resource.get_mem r in
+  match Memory.nth_error p m with
+  | None => None (* tried to access out of bounds *)
+  | Some q => (* get locked of qnode *)
+    let qnode_locked:bool := Qnode.get_locked q in
+    (* get local vars *)
+    let v:local_vars := State.get_vars s in
+    (* update env *)
+    Some (Env.set_state (State.set_vars (set_locked qnode_locked v) s) e)
+  end.
 
-      | WRITE_NEXT   : Vars.var -> Val.val -> act
-      | WRITE_LOCKED : Vars.var -> Val.val -> act
+(** [write_next to_write next e] will set the
+    field [qnode.next] of the [qnode] of the
+    index [to_write] to the value of [next]. *)
+Definition write_next (to_write:local_var) (next:expr) (e:env) : option env :=
+  (* get pid from [to_write] *)
+  let s:state := Env.get_state e in
+  match State.get_local_var_value to_write s with
+  | PID p => (* should be pid *)
+    (* get qnode *)
+    let r:resource := Env.get_resource e in
+    let m:mem := Resource.get_mem r in
+    match Memory.nth_error p m with
+    | None => None (* [qnode] must exist *)
+    | Some q =>
+      (* make sure [next] is a [VAL] *)
+      match eval next s with
+      | Some (VAL v) =>
+        (* check that this is some kind of nat *)
+        match valid_cast_to_nat v with
+        | (false, _) => None (* i.e., BOOL, NIL *)
+        | (true, None) => None (* i.e., INDEX NONE *)
+        | (true, Some n) =>
+          match Memory.nth_replace (Qnode.set_next (Some n) q) p m with
+          | None => None
+          | Some m => Some (Env.set_resource (Resource.set_mem m r) e)
+          end
+        end
+      | _ => None (* [next] must be an [VAL] *)
+      end
+    end
+  | _ => None (* [to_write] must be a [pid] *)
+  end.
 
-      | FETCH_AND_STORE  : act
-      | COMPARE_AND_SWAP : act
-      .
+(** [write_locked to_write locked e] will set the
+    field [qnode.locked] of the [qnode] of the
+    index [to_write] to the value of [locked]. *)
+Definition write_locked (to_write:local_var) (locked:expr) (e:env) : option env :=
+  (* get pid from [to_write] *)
+  let s:state := Env.get_state e in
+  match State.get_local_var_value to_write s with
+  | PID p => (* should be pid *)
+    (* get qnode *)
+    let r:resource := Env.get_resource e in
+    let m:mem := Resource.get_mem r in
+    match Memory.nth_error p m with
+    | None => None (* [qnode] must exist *)
+    | Some q =>
+      (* make sure [locked] is a [VAL] of [BOOL] *)
+      match eval locked s with
+      | Some (VAL (BOOL b)) =>
+        match Memory.nth_replace (Qnode.set_locked b q) p m with
+        | None => None
+        | Some m => Some (Env.set_resource (Resource.set_mem m r) e)
+        end
+      | _ => None (* [locked] must be an [VAL] of [BOOL] *)
+      end
+    end
+  | _ => None (* [to_write] must be a [pid] *)
+  end.
 
-    Inductive guard : (act * env) -> Prop :=
+Definition fetch_and_store (e:env) : option env :=
+  (* get [i] *)
+  let r:resource := Env.get_resource e in
+  let i:index := Resource.get_lock_i r in
+  (* store [i] in [predecessor] *)
+  let s:state := Env.get_state e in
+  let v:local_vars := State.get_vars s in
+  let v:local_vars := set_predecessor i v in
+  let s:state := State.set_vars v s in
+  (* set [i] to [pid] *)
+  let p:pid := State.get_pid s in
+  let r:resource := Resource.set_lock_i (Index.of_pid p) r in
+  (* update env *)
+  Some (s, r).
 
-      (* no guard. *)
-      | G_READ_NEXT : forall e,
-        guard (READ_NEXT, e)
 
-      (* check that [qnode.next] of [pid] is not None. *)
-      | G_READ_LOCKED : forall v b e,
-        (Memory._Get.next_of
-          (Index.of_pid (Env._Get.pid e))
-          (Env._Get.mem e))=v /\ v=(Some b) ->
-        guard (READ_LOCKED, e)
+Definition compare_and_swap (e:env) : option env :=
+  (* set [j] to [pid] *)
+  let s:state := Env.get_state e in
+  let p:pid := State.get_pid s in
+  let r:resource := Env.get_resource e in
+  let r:resource := Resource.set_lock_j (Index.of_pid p) r in
+  (* get [i] and [j] *)
+  let i:index := Resource.get_lock_i r in
+  let j:index := Resource.get_lock_j r in
+  (* if the same, then set [swap] to true and set [i] to [Nil], else false *)
+  let v:local_vars := State.get_vars s in
+  match Index.eqb i j with
+  | true =>
+    (* set [swap] true *)
+    let v:local_vars := set_swap true v in
+    let s:state := State.set_vars v s in
+    (* set [i] to [Nil] *)
+    let r:resource := Resource.set_lock_i Nil r in
+    (* update env *)
+    Some (s, r)
+  | false =>
+    (* set [swap] false *)
+    let v:local_vars := set_swap false v in
+    let s:state := State.set_vars v s in
+    (* update env *)
+    Some (s, r)
+  end.
 
-      (* check that [vqi] is not None. *)
-      | G_WRITE_NEXT : forall vqi qi vni ni e,
-        (Env._Get.var vqi e)=(Some qi) /\ (PID.is_pid qi)=true /\
-        (Env._Get.val vni e)=(Some ni) /\ (PID.is_pid ni)=true /\
-        vni=(Val.INDEX (Some ni)) ->
-        guard (WRITE_NEXT vqi vni, e)
 
-      (* check [vqi] and [vnl] are not None, and that [vnl] is Some ibool. *)
-      | G_WRITE_LOCKED : forall vqi qi vnl nl e,
-        (Env._Get.var vqi e)=(Some qi) /\ (PID.is_pid qi)=true     /\
-        (Env._Get.val vnl e)=(Some nl) /\ (IBool.is_ibool nl)=true /\
-        vnl=(Val.IBOOL (Some nl)) ->
-        guard (WRITE_LOCKED vqi vnl, e)
+Definition do_act (a:act) (e:env) : (tm*env) :=
+  match a with
+  | NCS   => (OK, e)
+  | ENTER => (OK, e)
+  | LEAVE => (OK, e)
 
-      (* no guard. *)
-      | G_FETCH_AND_STORE : forall e,
-        guard (FETCH_AND_STORE, e)
-
-      (* no guard. *)
-      | G_COMPARE_AND_SWAP : forall e,
-        guard (COMPARE_AND_SWAP, e)
-      .
-
-    Print guard.
-
-    Definition update_env (a:act) (e:env) : env :=
+  | _ =>
+    let res : option env :=
       match a with
-      (* CS Access *)
-      | NCS   => e
-      | ENTER => e
-      | LEAVE => e
+      | READ_NEXT   => read_next e
+      | READ_LOCKED => read_locked e
 
-      (* Memory Access *)
-      | READ_NEXT    => Env.Handle.read_next e
-      | READ_LOCKED  => Env.Handle.read_locked e
+      | WRITE_NEXT to_write next   => write_next to_write next e
+      | WRITE_LOCKED to_write next => write_locked to_write next e
 
-      | WRITE_NEXT to_write next =>
-          Env.Handle.write_next to_write next e
+      | FETCH_AND_STORE => fetch_and_store e
+      | COMPARE_AND_SWAP => compare_and_swap e
 
-      | WRITE_LOCKED to_write locked =>
-          Env.Handle.write_locked to_write locked e
-
-      (* Lock Access *)
-      | FETCH_AND_STORE  => Env.Handle.fetch_and_store e
-      | COMPARE_AND_SWAP => Env.Handle.compare_and_swap e
-
-      end.
-
-  End Operation.
-
-  Inductive tm : Type :=
-    | ERR : tm (* error *)
-    | OK  : tm (* no-op *)
-    | END : tm (* termination *)
-
-    | IF  : Expr.expr -> tm -> tm -> tm
-
-    | ACT : Operation.act -> tm
-
-    | SEQ : tm -> tm -> tm
-
-    | LOOP      : tm -> tm (* inner loop body -> *)
-    | LOOP_END  : tm
-
-    (* loop id -> body -> outer continuation -> ... *)
-    | LOOP_OVER : iloop -> tm -> tm -> tm
-    | BREAK     : iloop -> tm
-    .
-
-  (* following: https://softwarefoundations.cis.upenn.edu/plf-current/Types.html *)
-
-  Declare Custom Entry tm.
-  Declare Scope tm_scope.
-  Notation "<{ e }>" := e (e custom tm at level 99): tm_scope.
-  Notation "( x )" := x (in custom tm, x at level 99): tm_scope.
-  Notation "x" := x (in custom tm at level 0, x constr at level 0): tm_scope.
-  Notation "'if' c 'then' t 'else' e" := (IF c t e)
-                  (in custom tm at level 90, c custom tm at level 80,
-                    t custom tm at level 80, e custom tm at level 80): tm_scope.
-  Local Open Scope tm_scope.
-
-  Fixpoint subst (new old:tm) (loops:bool) : tm :=
-    match old with
-    | ERR => ERR
-    | OK   => OK
-    | END   => END
-
-    | IF c t e => IF c (subst new t loops) (subst new e loops)
-
-    | ACT a => ACT a
-
-    (* do not substitute in other body *)
-    | SEQ l r => SEQ l (subst new r loops)
-
-    | LOOP b   => if loops then LOOP (subst new b loops) else LOOP b
-    | LOOP_END => new
-
-    | LOOP_OVER l b c => LOOP_OVER l (subst new b loops) (subst new c loops)
-    | BREAK l         => BREAK l
-    end.
-
-  Module Semantics.
-
-    Inductive action : Type :=
-    | SILENT : action
-    | LABEL  : Operation.act -> pid -> action.
-
-    Reserved Notation "t '--<{' a '}>-->' t'" (at level 40).
-
-    Inductive step : (tm * env) -> action -> (tm * env) -> Prop :=
-
-      | ACT : forall a (e:env),
-        Operation.guard (a, e) ->
-        (ACT a, e) --<{LABEL a (Env._Get.pid e)}>--> (OK, Operation.update_env a e)
-
-      | SEQ : forall a l1 l2 r e1 e2,
-        (l1, e1) --<{a}>--> (l2, e2) ->
-        (SEQ l1 r, e1) --<{a}>--> (SEQ l2 r, e2)
-
-      | SEQ_END : forall r e,
-        (SEQ OK r, e) --<{SILENT}>--> (r, e)
-
-      | LOOP  : forall t e,
-        (LOOP t, e) --<{SILENT}>--> (subst t LOOP_END false, e)
-
-      | BREAK : forall l c e,
-        (LOOP_OVER l (BREAK l) c, e) --<{SILENT}>--> (c, e)
-
-      | LOOP_OVER : forall a l t1 t2 c e1 e2,
-        (LOOP t1, e1) --<{a}>--> (LOOP t2, e2) ->
-          (LOOP_OVER l t1 c, e1) --<{a}>--> (LOOP_OVER l t2 c, e2)
-
-      | IF_TT : forall t1 t2 e,
-        (<{ if Expr.TT then t1 else t2 }>, e) --<{SILENT}>--> (t1, e)
-
-      | IF_FF : forall t1 t2 e,
-        (<{ if Expr.FF then t1 else t2 }>, e) --<{SILENT}>--> (t2, e)
-
-      | IF : forall c1 c2 t1 t2 e,
-        (Expr.eval (c1, e) (c2, e)) ->
-        (<{ if c1 then t1 else t2 }>, e) --<{SILENT}>--> (<{ if c2 then t1 else t2 }>, e)
-
-    where "t '--<{' a '}>-->' t'" := (step t a t').
-
-  End Semantics.
-
-End Process.
+      | _ => None (* shouldn't happen, outer match catches these*)
+      end
+    in
+    match res with
+    | None => (ERR, e)
+    | Some e => (OK, e)
+    end
+  end.
 
 
-(*************************************************************************)
-(**** System (of processes) **********************************************)
-(*************************************************************************)
-Module System.
+Inductive action : Type :=
+  | SILENT : action
+  | LABEL  : act -> pid -> action.
 
-  Inductive sys : Type :=
-    | PRC : Process.tm -> State.local -> sys
-    | PAR : sys -> sys -> sys
-    | TERM : sys
-    .
+Reserved Notation "t '--<{' a '}>-->' t'" (at level 40).
 
-  Module LTS.
-    Reserved Notation "t '--<{' a '}>-->' t'" (at level 40).
-    Reserved Notation "t '==<{' a '}>==>' t'" (at level 40).
+Inductive step : (tm * env) -> action -> (tm * env) -> Prop :=
 
-    Inductive lts : sys * Resource.resource -> Process.Semantics.action -> sys * Resource.resource -> Prop :=
+  | STEP_ACT : forall a e,
+    (ACT a, e) --<{LABEL a (State.get_pid (Env.get_state e))}>--> (do_act a e)
 
-    (* wrapper for sharing global resource with local process. *)
-      | PRC : forall a t1 t2 s1 s2 r1 r2,
-        (t1, (s1, r1)) --<{a}>--> (t2, (s2, r2)) ->
-        (PRC t1 s1, r1) ==<{a}>==> (PRC t2 s2, r2)
+  | STEP_SEQ : forall a l1 l2 r e1 e2,
+    (l1, e1) --<{a}>--> (l2, e2) ->
+    (SEQ l1 r, e1) --<{a}>--> (SEQ l2 r, e2)
 
-      | PAR_L : forall a l1 l2 r gr1 gr2,
-        (l1, gr1) ==<{a}>==> (l2, gr2) ->
-        (PAR l1 r, gr1) ==<{a}>==> (PAR l2 r, gr2)
+  | STEP_SEQ_END : forall r e,
+    (SEQ OK r, e) --<{SILENT}>--> (r, e)
 
-      | PAR_R : forall a l r1 r2 gr1 gr2,
-        (r1, gr1) ==<{a}>==> (r2, gr2) ->
-        (PAR l r1, gr1) ==<{a}>==> (PAR l r2, gr2)
+  | STEP_LOOP  : forall t e,
+    (LOOP t, e) --<{SILENT}>--> (subst t LOOP_END false, e)
 
-      | END_L : forall a ls r gr,
-        (PAR (PRC Process.END ls) r, gr) ==<{a}>==> (r, gr)
+  | STEP_BREAK : forall l c e,
+    (LOOP_OVER l (BREAK l) c, e) --<{SILENT}>--> (c, e)
 
-      | END_R : forall a l rs gr,
-        (PAR l (PRC Process.END rs), gr) ==<{a}>==> (l, gr)
+  | STEP_LOOP_OVER : forall a l t1 t2 c e1 e2,
+    (LOOP t1, e1) --<{a}>--> (LOOP t2, e2) ->
+      (LOOP_OVER l t1 c, e1) --<{a}>--> (LOOP_OVER l t2 c, e2)
 
-      where "t '==<{' a '}>==>' t'" := (lts t a t')
-      and "t '--<{' a '}>-->' t'" := (Process.Semantics.step t a t').
+  | STEP_IF_TT : forall t1 t2 e,
+    (<{ if TRU then t1 else t2 }>, e) --<{SILENT}>--> (t1, e)
 
-    Print lts.
-  End LTS.
+  | STEP_IF_FF : forall t1 t2 e,
+    (<{ if FLS then t1 else t2 }>, e) --<{SILENT}>--> (t2, e)
 
-End System.
+  | STEP_IF : forall c t1 t2 s r,
+    (<{ if c then t1 else t2 }>, (s, r)) --<{SILENT}>--> (<{ if c (*(eval c s)*) then t1 else t2 }>, (s, r))
+
+  where "t '--<{' a '}>-->' t'" := (step t a t').
+
+
+
+
+
+Inductive sys : Type :=
+  | PRC : tm -> state -> sys
+  | PAR : sys -> sys -> sys
+  | TERM : sys
+  .
+
+Reserved Notation "t '==<{' a '}>==>' t'" (at level 40).
+
+Inductive lts : sys * resource -> action -> sys * resource -> Prop :=
+
+  | LTS_PRC : forall a t1 t2 s1 s2 r1 r2,
+    (t1, (s1, r1)) --<{a}>--> (t2, (s2, r2)) ->
+    (PRC t1 s1, r1) ==<{a}>==> (PRC t2 s2, r2)
+
+  | LTS_PAR_L : forall a l1 l2 r gr1 gr2,
+    (l1, gr1) ==<{a}>==> (l2, gr2) ->
+    (PAR l1 r, gr1) ==<{a}>==> (PAR l2 r, gr2)
+
+  | LTS_PAR_R : forall a l r1 r2 gr1 gr2,
+    (r1, gr1) ==<{a}>==> (r2, gr2) ->
+    (PAR l r1, gr1) ==<{a}>==> (PAR l r2, gr2)
+
+  | LTS_END_L : forall a ls r gr,
+    (PAR (PRC END ls) r, gr) ==<{a}>==> (r, gr)
+
+  | LTS_END_R : forall a l rs gr,
+    (PAR l (PRC END rs), gr) ==<{a}>==> (l, gr)
+
+  where "t '==<{' a '}>==>' t'" := (lts t a t')
+  and "t '--<{' a '}>-->' t'" := (step t a t').
+
 
 
 (*************************************************************************)
 (**** Example ************************************************************)
 (*************************************************************************)
 
-Import Process.
-Import Operation.
 Import Expr.
 
 Example Acquire : tm :=
-  SEQ (ACT (WRITE_NEXT Vars.PID Val.NIL)) (
+  SEQ (ACT (WRITE_NEXT VAR_PID (VAL NIL))) (
     SEQ (ACT FETCH_AND_STORE) (
-      IF (NOT (EQ (VAR Vars.PREDECESSOR) NIL)) (
-        SEQ (ACT (WRITE_LOCKED Vars.PREDECESSOR (Val.PID))) (
+      IF (NOT (EQ (VAR VAR_PREDECESSOR) (VAL NIL))) (
+        SEQ (ACT (WRITE_LOCKED VAR_PREDECESSOR (VAR VAR_PID))) (
           LOOP_OVER 0 (
             SEQ (ACT READ_LOCKED) (
-              IF (NOT (VAR Vars.LOCKED)) (BREAK 0) (OK)
+              IF (NOT (VAR VAR_LOCKED)) (BREAK 0) (OK)
             )
           ) (END)
         )
@@ -1032,17 +671,17 @@ Example Acquire : tm :=
 
 Example Release : tm :=
   SEQ (ACT READ_NEXT) (
-    IF (EQ NIL (VAR Vars.NEXT)) (
+    IF (EQ (VAL NIL) (VAR VAR_NEXT)) (
       SEQ (ACT COMPARE_AND_SWAP) (
-        IF (EQ FF (VAR Vars.SWAP)) (
+        IF (EQ FLS (VAR VAR_SWAP)) (
           LOOP_OVER 0 (*L*) (
             SEQ (ACT READ_NEXT) (
-              IF (NOT (EQ NIL (VAR Vars.NEXT))) (BREAK 0 (*L*)) (OK)
+              IF (NOT (EQ (VAL NIL) (VAR VAR_NEXT))) (BREAK 0 (*L*)) (OK)
             )
-          ) (ACT (WRITE_LOCKED Vars.NEXT Val.TRU))
+          ) (ACT (WRITE_LOCKED VAR_NEXT TRU))
         ) (END)
       )
-    ) (ACT (WRITE_LOCKED Vars.NEXT Val.FLS))
+    ) (ACT (WRITE_LOCKED VAR_NEXT FLS))
   ).
 
 
@@ -1060,15 +699,22 @@ Example P : tm :=
   ).
 
 
-Example p0 : tm * env := (P, (State.create 0, Resource.initial 0)).
-MeBi LTS Semantics.step p0.
+
+(**********************************)
+(**** Single process **************)
+(**********************************)
+
+Example p0 : tm * env := (P, (State.initial, Resource.initial 0)).
+MeBi LTS step p0.
 
 
-(*******************************)
-(**** As part of a system ******)
-(*******************************)
 
-Definition process : Type := tm * State.local.
+(**********************************)
+(**** System **********************)
+(**********************************)
+
+Definition process : Type := tm * state.
+
 Definition spawn (p:pid) (b:tm) : process := (b, State.create p).
 
 Fixpoint populate (n:nat) (b:tm) : list process :=
@@ -1077,23 +723,25 @@ Fixpoint populate (n:nat) (b:tm) : list process :=
   | S m => app (populate m b) [spawn n b]
   end.
 
-Definition system : Type := list process * Resource.resource.
+Definition system : Type := list process * resource.
+
 Definition create (n:nat) (b:tm) : system := (populate n b, Resource.initial n).
 
-Fixpoint load (ps:list process) : System.sys :=
+Fixpoint load (ps:list process) : sys :=
   match ps with
-  | [] => System.TERM
+  | [] => TERM
   | h :: t =>
     match h with
-    | (p, s) => System.PAR (System.PRC p s) (load t)
+    | (p, s) => PAR (PRC p s) (load t)
     end
   end.
 
-Definition composition : Type := System.sys * Resource.resource.
+Definition composition : Type := sys * resource.
 Definition compose (s:system) : composition :=
   match s with
   | (ps, r) => (load ps, r)
   end.
 
 Example ncs : composition := compose (create 5 P).
-MeBi LTS System.LTS.lts ncs.
+MeBi LTS lts ncs.
+
